finish heaplang notation

Test/HeapLang.lean
@@ -120,9 +120,14 @@ instance : Coe Nat BaseLit where
 instance : Coe Int BaseLit where
   coe n := .int n
 
+instance : Coe Bool BaseLit where
+  coe b := .bool b
+
 instance : Coe Unit BaseLit where
   coe _ := .unit
 
+/- TODO: this instance is sometimes not reduced away. What can we do about this? -/
+@[reducible]
 instance {n} : OfNat BaseLit n where
   ofNat := .int n
 
@@ -385,33 +390,142 @@ def Exp.denote (e : Exp) : ITree heaplangE Val :=
     fail "prophecy is not implemented"
 partial_fixpoint
 
+
+section Derived
+def Exp.stuck : Exp := Exp.app (.val $ .lit $ .int 0) (.val $ .lit $ .int 0)
+
+@[simp]
+theorem Exp.stuck_subst x v:
+  Exp.substStr x v Exp.stuck = Exp.stuck := by
+  simp [Exp.stuck, Exp.substStr]
+
+def Exp.assert (e : Exp) := Exp.if e (.val $ .lit .unit) Exp.stuck
+
+@[simp]
+theorem Exp.assert_subst x v e:
+  Exp.substStr x v (Exp.assert e) = Exp.assert (Exp.substStr x v e) := by
+  simp [Exp.assert, Exp.substStr]
+end Derived
+
 section Notation
 open Lean Lean.PrettyPrinter Elab Parser
 
 declare_syntax_cat hl_exp
 declare_syntax_cat hl_val
 
+/-- embedding heaplang expressions into terms -/
 syntax:max "hl(" hl_exp ")" : term
+/-- embedding heaplang binders into terms -/
 syntax:max "hl_binder(" binderIdent ")" : term
+/-- embedding heaplang values into terms -/
 syntax:max "hl_val(" hl_val ")" : term
-syntax:max "(" hl_exp ")" : hl_exp
-syntax:max "v(" hl_val ")" : hl_exp
-syntax:max "{" term "}" : hl_exp
-syntax:max "{" term "}" : hl_val
-syntax:max ident : hl_val
-syntax:max "#" term:max : hl_exp
-syntax:max "#" term:max : hl_val
-syntax:max ident : hl_exp
-syntax:65 hl_exp:66 " + " hl_exp:65 : hl_exp
-syntax:60 hl_exp:61 " = " hl_exp:60 : hl_exp
 
-syntax:100 hl_exp:100 ppSpace hl_exp:101 : hl_exp -- app
+/-- escaping -/
+syntax:max "{" term "}" : hl_val
+/-- escaping identifiers -/
+syntax:max ident : hl_val
+/-- embedding literals -/
+syntax:max "#" term:max : hl_val
+/-- pairs -/
+syntax:max "(" hl_val ", " hl_val,+ ")" : hl_val
+/-- injL -/
+syntax:100 "injl(" hl_val ")" : hl_val
+/-- injR -/
+syntax:100 "injr(" hl_val ")" : hl_val
+
+/-- parenthesis -/
+syntax:max "(" hl_exp ")" : hl_exp
+/-- embedding values -/
+syntax:max "v(" hl_val ")" : hl_exp
+/-- escaping -/
+syntax:max "{" term "}" : hl_exp
+/-- embedding literals -/
+syntax:max "#" term:max : hl_exp
+/-- variables -/
+syntax:max ident : hl_exp
+-- levels are taken from https://github.com/leanprover/lean4/blob/985f350dcd18fc7814dfa677cac09933f44f3215/src/Init/Notation.lean#L280
+/-- addition -/
+syntax:65 hl_exp:66 " + " hl_exp:65 : hl_exp
+/-- offset -/
+syntax:65 hl_exp:66 " +ₗ " hl_exp:65 : hl_exp
+/-- subtraction -/
+syntax:65 hl_exp:66 " - " hl_exp:65 : hl_exp
+/-- multiplication -/
+syntax:70 hl_exp:71 " * " hl_exp:70 : hl_exp
+/-- division -/
+syntax:70 hl_exp:71 " / " hl_exp:70 : hl_exp
+/-- modulo -/
+syntax:70 hl_exp:71 " % " hl_exp:70 : hl_exp
+/-- and -/
+syntax:60 hl_exp:61 " & " hl_exp:60 : hl_exp
+/-- or -/
+syntax:55 hl_exp:56 " | " hl_exp:55 : hl_exp
+/-- xor -/
+syntax:58 hl_exp:59 " ^ " hl_exp:58 : hl_exp
+/-- shiftl -/
+syntax:75 hl_exp:76 " <<< " hl_exp:75 : hl_exp
+/-- shiftr -/
+syntax:75 hl_exp:76 " >>> " hl_exp:75 : hl_exp
+/-- le -/
+syntax:50 hl_exp:50 " <= " hl_exp:50 : hl_exp
+syntax:50 hl_exp:50 " ≤ " hl_exp:50 : hl_exp
+/-- lt -/
+syntax:50 hl_exp:50 " < " hl_exp:50 : hl_exp
+/-- equality -/
+syntax:50 hl_exp:50 " = " hl_exp:50 : hl_exp
+
+/-- neg -/
+syntax:100 "~" hl_exp:100 : hl_exp
+/-- minus -/
+syntax:75 "-" hl_exp:75 : hl_exp
+
+/-- if -/
+syntax:10 "if " hl_exp:10 " then " hl_exp:10 " else " hl_exp:10 : hl_exp
+
+/-- application -/
+syntax:100 hl_exp:100 ppSpace hl_exp:101 : hl_exp
+/-- let -/
 syntax:10 "let " binderIdent " := " hl_exp:10 "; " hl_exp:1 : hl_exp
+/-- sequencing -/
 syntax:5 hl_exp:6 "; " hl_exp:5 : hl_exp
+/-- lambda -/
 syntax:10 "λ " binderIdent+ ", " hl_exp:10 : hl_exp
+/-- lambda -/
 syntax:10 "λ " binderIdent+ ", " hl_exp:10 : hl_val
+/-- recursive function -/
 syntax:10 "rec " binderIdent ppSpace binderIdent+ " := " hl_exp:10 : hl_exp
+/-- recursive function -/
 syntax:10 "rec " binderIdent ppSpace binderIdent+ " := " hl_exp:10 : hl_val
+
+/-- pairs -/
+syntax:max "(" hl_exp ", " hl_exp,+ ")" : hl_exp
+/-- fst -/
+syntax:100 "fst(" hl_exp ")" : hl_exp
+/-- snd -/
+syntax:100 "snd(" hl_exp ")" : hl_exp
+
+/-- case -/
+syntax:100 "case: " hl_exp:80 " | " binderIdent " => " hl_exp:80 " | " binderIdent " => " hl_exp:80 : hl_exp
+/-- injL -/
+syntax:100 "injl(" hl_exp ")" : hl_exp
+/-- injR -/
+syntax:100 "injr(" hl_exp ")" : hl_exp
+
+/-- heap operations -/
+syntax:100 "allocn(" hl_exp ", " hl_exp ")" : hl_exp
+syntax:100 "ref(" hl_exp ")" : hl_exp
+syntax:100 "free(" hl_exp ")" : hl_exp
+syntax:80 "!" hl_exp:80 : hl_exp
+syntax:80 hl_exp:80 " ← " hl_exp:80 : hl_exp
+syntax:100 "cmpXchg(" hl_exp ", " hl_exp ", " hl_exp ")" : hl_exp
+syntax:100 "xchg(" hl_exp ", " hl_exp ")" : hl_exp
+syntax:100 "faa(" hl_exp ", " hl_exp ")" : hl_exp
+
+/-- fork -/
+syntax:100 "fork(" hl_exp  ")" : hl_exp
+
+/-- assert -/
+syntax:100 "assert(" hl_exp  ")" : hl_exp
 
 partial def unpackHLExp [Monad m] [MonadRef m] [MonadQuotation m] : Term → m (TSyntax `hl_exp)
   | `(hl($e)) => `(hl_exp|$e)
@@ -426,10 +540,12 @@ partial def unpackHLBinder [Monad m] [MonadRef m] [MonadQuotation m] : Term → 
 -- TODO
   | `($_) => panic! "unknown binder"
 
+/-- elaborating binders -/
 macro_rules
   | `(hl_binder(_)) => `(Binder.anon)
   | `(hl_binder($i:ident)) => `(Binder.named $(Syntax.mkStrLit i.getId.toString))
 
+/-- elaborating values -/
 macro_rules
   | `(hl_val($i:ident)) => pure i
   | `(hl_val({$t})) => pure t
@@ -437,22 +553,61 @@ macro_rules
   | `(hl_val(rec $f $x := $e)) => do `(Val.rec_ hl_binder($f) hl_binder($x) hl($e))
   | `(hl_val(rec $f $x $xs* := $e)) => do `(hl_val(rec $f $x := λ $xs*, $e))
   | `(hl_val(λ $xs*, $e)) => do `(hl_val(rec _ $xs* := $e))
+  | `(hl_val(($e1, $e2))) => `(Val.pair hl_val($e1) hl_val($e2))
+  | `(hl_val(($e1, $e2, $e3,*))) => `(hl_val(($e1, ($e2, $e3,*))))
+  | `(hl_val(injl($e1))) => `(Val.injL hl_val($e1))
+  | `(hl_val(injr($e1))) => `(Val.injR hl_val($e1))
 
+/-- elaborating expressions -/
 macro_rules
   | `(hl(($e))) => `(hl($e))
   | `(hl({$t})) => pure t
   | `(hl(v($e))) => `(Exp.val hl_val($e))
   | `(hl(# $e)) => `(hl(v(# $e)))
   | `(hl($i:ident)) => `(Exp.var $(Syntax.mkStrLit i.getId.toString))
-  | `(hl($e1 + $e2)) => `(Exp.binop .plus hl($e1) hl($e2))
-  | `(hl($e1 = $e2)) => `(Exp.binop .eq hl($e1) hl($e2))
+  | `(hl($e1 + $e2)) => `(Exp.binop BinOp.plus hl($e1) hl($e2))
+  | `(hl($e1 +ₗ $e2)) => `(Exp.binop BinOp.offset hl($e1) hl($e2))
+  | `(hl($e1 - $e2)) => `(Exp.binop BinOp.minus hl($e1) hl($e2))
+  | `(hl($e1 * $e2)) => `(Exp.binop BinOp.mult hl($e1) hl($e2))
+  | `(hl($e1 / $e2)) => `(Exp.binop BinOp.tdiv hl($e1) hl($e2))
+  | `(hl($e1 % $e2)) => `(Exp.binop BinOp.tmod hl($e1) hl($e2))
+  | `(hl($e1 & $e2)) => `(Exp.binop BinOp.and hl($e1) hl($e2))
+  | `(hl($e1 | $e2)) => `(Exp.binop BinOp.or hl($e1) hl($e2))
+  | `(hl($e1 ^ $e2)) => `(Exp.binop BinOp.xor hl($e1) hl($e2))
+  | `(hl($e1 <<< $e2)) => `(Exp.binop BinOp.shiftl hl($e1) hl($e2))
+  | `(hl($e1 >>> $e2)) => `(Exp.binop BinOp.shiftr hl($e1) hl($e2))
+  | `(hl($e1 <= $e2)) => `(hl($e1 ≤ $e2))
+  | `(hl($e1 ≤ $e2)) => `(Exp.binop BinOp.le hl($e1) hl($e2))
+  | `(hl($e1 < $e2)) => `(Exp.binop BinOp.lt hl($e1) hl($e2))
+  | `(hl($e1 = $e2)) => `(Exp.binop BinOp.eq hl($e1) hl($e2))
+  | `(hl(~$e1)) => `(Exp.unop UnOp.neg hl($e1))
+  | `(hl(-$e1)) => `(Exp.unop UnOp.minus hl($e1))
+  | `(hl(if $e1 then $e2 else $e3)) => `(Exp.if hl($e1) hl($e2) hl($e3))
   | `(hl($e1 $e2)) => `(Exp.app hl($e1) hl($e2))
   | `(hl(rec $f $x := $e)) => do `(Exp.rec_ hl_binder($f) hl_binder($x) hl($e))
   | `(hl(rec $f $x $xs* := $e)) => do `(hl(rec $f $x := λ $xs*, $e))
   | `(hl(λ $xs*, $e)) => do `(hl(rec _ $xs* := $e))
   | `(hl($e1; $e2)) => `(hl(let _ := $e1; $e2))
   | `(hl(let $i := $e1; $e2)) => `(hl((λ $i, $e2) $e1))
+  | `(hl(($e1, $e2))) => `(Exp.pair hl($e1) hl($e2))
+  | `(hl(($e1, $e2, $e3,*))) => `(hl(($e1, ($e2, $e3,*))))
+  | `(hl(fst($e1))) => `(Exp.fst hl($e1))
+  | `(hl(snd($e1))) => `(Exp.snd hl($e1))
+  | `(hl(case: $e1 | $i2 => $e2 | $i3 => $e3)) => `(Exp.case hl($e1) hl(λ $i2, $e2) hl(λ $i3, $e3))
+  | `(hl(injl($e1))) => `(Exp.injL hl($e1))
+  | `(hl(injr($e1))) => `(Exp.injR hl($e1))
+  | `(hl(allocn($e1, $e2))) => `(Exp.allocN hl($e1) hl($e2))
+  | `(hl(ref($e1))) => `(hl(allocn(#1, $e1)))
+  | `(hl(free($e1))) => `(Exp.free hl($e1))
+  | `(hl(! $e1)) => `(Exp.load hl($e1))
+  | `(hl($e1 ← $e2)) => `(Exp.store hl($e1) hl($e2))
+  | `(hl(cmpXchg($e1, $e2, $e3))) => `(Exp.cmpXchg hl($e1) hl($e2) hl($e3))
+  | `(hl(xchg($e1, $e2))) => `(Exp.xchg hl($e1) hl($e2))
+  | `(hl(faa($e1, $e2))) => `(Exp.faa hl($e1) hl($e2))
+  | `(hl(fork($e1))) => `(Exp.fork hl($e1))
+  | `(hl(assert($e1))) => `(Exp.assert hl($e1))
 
+/-- delaborating Binders -/
 @[app_unexpander Binder.anon]
 def unexpAnon : Unexpander
   | `($_) => `(hl_binder(_))
@@ -462,23 +617,57 @@ def unexpNamed : Unexpander
   | `($_ $s:str) => `(hl_binder($(Lean.mkIdent $ Name.mkSimple s.getString):ident))
   | _ => throw ()
 
+/-- delaborating values -/
 @[app_unexpander Val.lit]
 def unexpLit : Unexpander
   | `($_ $arg) => `(hl_val(# $arg))
   | _ => throw ()
 
-partial def unexpValLit : TSyntax `hl_exp → UnexpandM (TSyntax `hl_exp)
-  | `(hl_exp | v(# $l)) => do
-    unexpValLit $ ← `(hl_exp | # $l)
-  | `(hl_exp | v({$i:ident})) => do
-    unexpValLit $ ← `(hl_exp | v($i:ident))
+partial def unexpLamVal : Term → UnexpandM Term
+  | `(hl_val(rec _ $x := $e)) => do
+    unexpLamVal $ ← `(hl_val(λ $x, $e))
+  | `(hl_val(λ $x, (λ $ys*, $e))) => do
+    unexpLamVal $ ← `(hl_val(λ $x $ys*, $e))
+  | x => return x
+
+@[app_unexpander Val.rec_]
+def unexpRecVal : Unexpander
+  | `($_ $f $x $e) => do
+    unexpLamVal $ ← `(hl_val(rec $(← unpackHLBinder f) $(← unpackHLBinder x) := $(← unpackHLExp e)))
+  | _ => throw ()
+
+partial def unexpPairVal' : Term → UnexpandM Term
+  | `(hl_val(($e1, ($e2, $e3,*)))) => do
+    unexpPairVal' $ ← `(hl_val(($e1, $e2, $e3,*)))
+  | x => return x
+
+@[app_unexpander Val.pair]
+def unexpPairVal : Unexpander
+  | `($_ $e1 $e2) => do
+    unexpPairVal' $ ← `(hl_val(($(← unpackHLVal e1), $(← unpackHLVal e2))))
+  | _ => throw ()
+
+@[app_unexpander Val.injL]
+def unexpInjlVal : Unexpander
+  | `($_ $e1) => do `(hl_val(injl($(← unpackHLVal e1))))
+  | _ => throw ()
+
+@[app_unexpander Val.injR]
+def unexpInjrVal : Unexpander
+  | `($_ $e1) => do `(hl_val(injr($(← unpackHLVal e1))))
+  | _ => throw ()
+
+/-- delaborating expressions -/
+partial def unexpValLit : Term → UnexpandM Term
+  | `(hl(v(# $l))) => do
+    unexpValLit $ ← `(hl(# $l))
+  | `(hl(v({$i:ident}))) => do
+    unexpValLit $ ← `(hl(v($i:ident)))
   | x => return x
 
 @[app_unexpander Exp.val]
 def unexpVal : Unexpander
-  | `($_ $arg) => do
-    let r ← unexpValLit $ ← `(hl_exp|v($(← unpackHLVal arg)))
-    `(hl($r))
+  | `($_ $arg) => do unexpValLit $ ← `(hl(v($(← unpackHLVal arg))))
   | _ => throw ()
 
 
@@ -490,52 +679,143 @@ def unexpVar : Unexpander
 @[app_unexpander Exp.binop]
 def unexpBinop : Unexpander
   | `($_ BinOp.plus $e1 $e2) => do `(hl(($(← unpackHLExp e1) + $(← unpackHLExp e2))))
+  | `($_ BinOp.offset $e1 $e2) => do `(hl(($(← unpackHLExp e1) +ₗ $(← unpackHLExp e2))))
+  | `($_ BinOp.minus $e1 $e2) => do `(hl(($(← unpackHLExp e1) - $(← unpackHLExp e2))))
+  | `($_ BinOp.mult $e1 $e2) => do `(hl(($(← unpackHLExp e1) * $(← unpackHLExp e2))))
+  | `($_ BinOp.tdiv $e1 $e2) => do `(hl(($(← unpackHLExp e1) / $(← unpackHLExp e2))))
+  | `($_ BinOp.tmod $e1 $e2) => do `(hl(($(← unpackHLExp e1) % $(← unpackHLExp e2))))
+  | `($_ BinOp.and $e1 $e2) => do `(hl(($(← unpackHLExp e1) & $(← unpackHLExp e2))))
+  | `($_ BinOp.or $e1 $e2) => do `(hl(($(← unpackHLExp e1) | $(← unpackHLExp e2))))
+  | `($_ BinOp.xor $e1 $e2) => do `(hl(($(← unpackHLExp e1) ^ $(← unpackHLExp e2))))
+  | `($_ BinOp.shiftl $e1 $e2) => do `(hl(($(← unpackHLExp e1) <<< $(← unpackHLExp e2))))
+  | `($_ BinOp.shiftr $e1 $e2) => do `(hl(($(← unpackHLExp e1) >>> $(← unpackHLExp e2))))
+  | `($_ BinOp.le $e1 $e2) => do `(hl(($(← unpackHLExp e1) ≤ $(← unpackHLExp e2))))
+  | `($_ BinOp.lt $e1 $e2) => do `(hl(($(← unpackHLExp e1) < $(← unpackHLExp e2))))
   | `($_ BinOp.eq $e1 $e2) => do `(hl(($(← unpackHLExp e1) = $(← unpackHLExp e2))))
   | _ => throw ()
 
-partial def unexpLam : TSyntax `hl_exp → UnexpandM (TSyntax `hl_exp)
-  | `(hl_exp | (rec _ $x := $e)) => do
-    unexpLam $ ← `(hl_exp | (λ $x, $e))
-  | `(hl_exp | (λ $x, (λ $ys, $e))) => do
-    unexpLam $ ← `(hl_exp | (λ $x $ys, $e))
+@[app_unexpander Exp.unop]
+def unexpUnop : Unexpander
+  | `($_ UnOp.neg $e1) => do `(hl((~$(← unpackHLExp e1))))
+  | `($_ UnOp.minus $e1) => do `(hl((-$(← unpackHLExp e1))))
+  | _ => throw ()
+
+@[app_unexpander Exp.if]
+def unexpIf : Unexpander
+  | `($_ $e1 $e2 $e3) => do `(hl(if $(← unpackHLExp e1) then $(← unpackHLExp e2) else $(← unpackHLExp e3) ))
+  | _ => throw ()
+
+partial def unexpLam : Term → UnexpandM Term
+  | `(hl((rec _ $x := $e))) => do
+    unexpLam $ ← `(hl((λ $x, $e)))
+  | `(hl((λ $x, (λ $ys*, $e)))) => do
+    unexpLam $ ← `(hl((λ $x $ys*, $e)))
   | x => return x
 
 @[app_unexpander Exp.rec_]
 def unexpRec : Unexpander
   | `($_ $f $x $e) => do
-    let r ← unexpLam $ ← `(hl_exp|(rec $(← unpackHLBinder f) $(← unpackHLBinder x) := $(← unpackHLExp e)))
-    `(hl($r))
+    unexpLam $ ← `(hl((rec $(← unpackHLBinder f) $(← unpackHLBinder x) := $(← unpackHLExp e))))
   | _ => throw ()
 
-partial def unexpLamVal : TSyntax `hl_val → UnexpandM (TSyntax `hl_val)
-  | `(hl_val | rec _ $x := $e) => do
-    unexpLamVal $ ← `(hl_val | λ $x, $e)
-  | `(hl_val | λ $x, (λ $ys, $e)) => do
-    unexpLamVal $ ← `(hl_val | λ $x $ys, $e)
-  | x => return x
-
-@[app_unexpander Val.rec_]
-def unexpRecVal : Unexpander
-  | `($_ $f $x $e) => do
-    let r ← unexpLamVal $ ← `(hl_val|rec $(← unpackHLBinder f) $(← unpackHLBinder x) := $(← unpackHLExp e))
-    `(hl_val($r))
-  | _ => throw ()
-
-partial def unexpLet : TSyntax `hl_exp → UnexpandM (TSyntax `hl_exp)
-  | `(hl_exp | (λ $f, $e2) $e1) => do
-    unexpLet $ ← `(hl_exp | let $f := $e1; $e2)
-  | `(hl_exp | let _ := $e1; $e2) => do
-    `(hl_exp | $e1; $e2)
+partial def unexpLet : Term → UnexpandM Term
+  | `(hl((λ $f, $e2) $e1)) => do
+    unexpLet $ ← `(hl(let $f := $e1; $e2))
+  | `(hl(let _ := $e1; $e2)) => do `(hl($e1; $e2))
   | x => return x
 
 @[app_unexpander Exp.app]
 def unexpApp : Unexpander
   | `($_ $e1 $e2) => do
-    let r ← unexpLet $ ← `(hl_exp|$(← unpackHLExp e1) $(← unpackHLExp e2))
-    `(hl($r))
+    unexpLet $ ← `(hl($(← unpackHLExp e1) $(← unpackHLExp e2)))
   | _ => throw ()
 
+partial def unexpPair' : Term → UnexpandM Term
+  | `(hl(($e1, ($e2, $e3,*)))) => do
+    unexpPair' $ ← `(hl(($e1, $e2, $e3,*)))
+  | x => return x
 
+@[app_unexpander Exp.pair]
+def unexpPair : Unexpander
+  | `($_ $e1 $e2) => do
+    unexpPair' $ ← `(hl(($(← unpackHLExp e1), $(← unpackHLExp e2))))
+  | _ => throw ()
+
+@[app_unexpander Exp.fst]
+def unexpFst : Unexpander
+  | `($_ $e1) => do `(hl(fst($(← unpackHLExp e1))))
+  | _ => throw ()
+
+@[app_unexpander Exp.snd]
+def unexpSnd : Unexpander
+  | `($_ $e1) => do `(hl(snd($(← unpackHLExp e1))))
+  | _ => throw ()
+
+@[app_unexpander Exp.injL]
+def unexpInjl : Unexpander
+  | `($_ $e1) => do `(hl(injl($(← unpackHLExp e1))))
+  | _ => throw ()
+
+@[app_unexpander Exp.injR]
+def unexpInjr : Unexpander
+  | `($_ $e1) => do `(hl(injr($(← unpackHLExp e1))))
+  | _ => throw ()
+
+@[app_unexpander Exp.case]
+def unexpCase : Unexpander
+  | `($_ $e1 hl((λ $i2, $e2)) hl((λ $i3, $e3))) => do `(hl(case: $(← unpackHLExp e1) | $i2 => $e2 | $i3 => $e3))
+  | _ => throw ()
+
+partial def unexpRef : Term → UnexpandM Term
+  | `(hl(allocn(#1, $e2))) => do `(hl(ref($e2)))
+  | x => return x
+
+@[app_unexpander Exp.allocN]
+def unexpAllocN : Unexpander
+  | `($_ $e1 $e2) => do unexpRef $ ← `(hl(allocn($(← unpackHLExp e1), $(← unpackHLExp e2))))
+  | _ => throw ()
+
+@[app_unexpander Exp.free]
+def unexpFree : Unexpander
+  | `($_ $e1) => do `(hl(free($(← unpackHLExp e1))))
+  | _ => throw ()
+
+@[app_unexpander Exp.load]
+def unexpLoad : Unexpander
+  | `($_ $e1) => do `(hl(!$(← unpackHLExp e1)))
+  | _ => throw ()
+
+@[app_unexpander Exp.store]
+def unexpStore : Unexpander
+  | `($_ $e1 $e2) => do `(hl($(← unpackHLExp e1) ← $(← unpackHLExp e2)))
+  | _ => throw ()
+
+@[app_unexpander Exp.cmpXchg]
+def unexpCmpXChg : Unexpander
+  | `($_ $e1 $e2 $e3) => do `(hl(cmpXchg($(← unpackHLExp e1), $(← unpackHLExp e2), $(← unpackHLExp e3))))
+  | _ => throw ()
+
+@[app_unexpander Exp.xchg]
+def unexpXChg : Unexpander
+  | `($_ $e1 $e2) => do `(hl(xchg($(← unpackHLExp e1), $(← unpackHLExp e2))))
+  | _ => throw ()
+
+@[app_unexpander Exp.faa]
+def unexpFAA : Unexpander
+  | `($_ $e1 $e2) => do `(hl(faa($(← unpackHLExp e1), $(← unpackHLExp e2))))
+  | _ => throw ()
+
+@[app_unexpander Exp.fork]
+def unexpFork : Unexpander
+  | `($_ $e1) => do `(hl(fork($(← unpackHLExp e1))))
+  | _ => throw ()
+
+@[app_unexpander Exp.assert]
+def unexpAssert : Unexpander
+  | `($_ $e1) => do `(hl(assert($(← unpackHLExp e1))))
+  | _ => throw ()
+
+section test
 variable (v : Val)
 /-- info: hl((#1 + (#1 + v(v)))) : Exp -/
 #guard_msgs in
@@ -567,13 +847,13 @@ info: Exp.binop BinOp.eq (Exp.val (Val.lit (@OfNat.ofNat BaseLit (nat_lit 1) (@i
 set_option pp.explicit true in
 #check hl(#1 = v + v(v))
 
-/-- info: hl((λ x y, #1)) : Exp -/
+/-- info: hl((λ x y z, #1)) : Exp -/
 #guard_msgs in
-#check hl(λ x y, #1)
+#check hl(λ x y z, #1)
 
-/-- info: hl_val(λ x y, #1) : Val -/
+/-- info: hl_val(λ x y z, #1) : Val -/
 #guard_msgs in
-#check hl_val(λ x y, #1)
+#check hl_val(λ x y z, #1)
 
 /--
 info: Exp.rec_ Binder.anon (Binder.named "x")
@@ -612,3 +892,139 @@ info: Exp.rec_ Binder.anon (Binder.named "x")
 #guard_msgs in
 set_option pp.explicit true in
 #check hl(λ x y, let z := #1; #2; x + y + z)
+
+/--
+info: hl((λ x y,
+      ((((#1 + (#2 +ₗ (#3 - (#4 * (#5 / (#6 % #7)))))) & #8) | (#9 ^ (#10 <<< (#11 >>> #12)))) ≤
+          (#13 ≤ (#14 < (#15 = (#16 + ((-#17) + (~#18))))))))) : Exp
+-/
+#guard_msgs in
+#check hl(λ x y, #1 + #2 +ₗ #3 - #4 * #5 / #6 % #7 & #8 | #9 ^ #10 <<< #11 >>> #12 <= #13 ≤ #14 < #15 = #16 + (-#17) + (~#18))
+
+/--
+info: Exp.rec_ Binder.anon (Binder.named "x")
+  (Exp.rec_ Binder.anon (Binder.named "y")
+    (Exp.binop BinOp.le
+      (Exp.binop BinOp.or
+        (Exp.binop BinOp.and
+          (Exp.binop BinOp.plus (Exp.val (Val.lit (@OfNat.ofNat BaseLit (nat_lit 1) (@instOfNatBaseLit (nat_lit 1)))))
+            (Exp.binop BinOp.offset
+              (Exp.val (Val.lit (@OfNat.ofNat BaseLit (nat_lit 2) (@instOfNatBaseLit (nat_lit 2)))))
+              (Exp.binop BinOp.minus
+                (Exp.val (Val.lit (@OfNat.ofNat BaseLit (nat_lit 3) (@instOfNatBaseLit (nat_lit 3)))))
+                (Exp.binop BinOp.mult
+                  (Exp.val (Val.lit (@OfNat.ofNat BaseLit (nat_lit 4) (@instOfNatBaseLit (nat_lit 4)))))
+                  (Exp.binop BinOp.tdiv
+                    (Exp.val (Val.lit (@OfNat.ofNat BaseLit (nat_lit 5) (@instOfNatBaseLit (nat_lit 5)))))
+                    (Exp.binop BinOp.tmod
+                      (Exp.val (Val.lit (@OfNat.ofNat BaseLit (nat_lit 6) (@instOfNatBaseLit (nat_lit 6)))))
+                      (Exp.val (Val.lit (@OfNat.ofNat BaseLit (nat_lit 7) (@instOfNatBaseLit (nat_lit 7)))))))))))
+          (Exp.val (Val.lit (@OfNat.ofNat BaseLit (nat_lit 8) (@instOfNatBaseLit (nat_lit 8))))))
+        (Exp.binop BinOp.xor (Exp.val (Val.lit (@OfNat.ofNat BaseLit (nat_lit 9) (@instOfNatBaseLit (nat_lit 9)))))
+          (Exp.binop BinOp.shiftl
+            (Exp.val (Val.lit (@OfNat.ofNat BaseLit (nat_lit 10) (@instOfNatBaseLit (nat_lit 10)))))
+            (Exp.binop BinOp.shiftr
+              (Exp.val (Val.lit (@OfNat.ofNat BaseLit (nat_lit 11) (@instOfNatBaseLit (nat_lit 11)))))
+              (Exp.val (Val.lit (@OfNat.ofNat BaseLit (nat_lit 12) (@instOfNatBaseLit (nat_lit 12)))))))))
+      (Exp.binop BinOp.le (Exp.val (Val.lit (@OfNat.ofNat BaseLit (nat_lit 13) (@instOfNatBaseLit (nat_lit 13)))))
+        (Exp.binop BinOp.lt (Exp.val (Val.lit (@OfNat.ofNat BaseLit (nat_lit 14) (@instOfNatBaseLit (nat_lit 14)))))
+          (Exp.binop BinOp.eq (Exp.val (Val.lit (@OfNat.ofNat BaseLit (nat_lit 15) (@instOfNatBaseLit (nat_lit 15)))))
+            (Exp.binop BinOp.plus
+              (Exp.val (Val.lit (@OfNat.ofNat BaseLit (nat_lit 16) (@instOfNatBaseLit (nat_lit 16)))))
+              (Exp.binop BinOp.plus
+                (Exp.unop UnOp.minus
+                  (Exp.val (Val.lit (@OfNat.ofNat BaseLit (nat_lit 17) (@instOfNatBaseLit (nat_lit 17))))))
+                (Exp.unop UnOp.neg
+                  (Exp.val (Val.lit (@OfNat.ofNat BaseLit (nat_lit 18) (@instOfNatBaseLit (nat_lit 18))))))))))))) : Exp
+-/
+#guard_msgs in
+set_option pp.explicit true in
+#check hl(λ x y, #1 + #2 +ₗ #3 - #4 * #5 / #6 % #7 & #8 | #9 ^ #10 <<< #11 >>> #12 <= #13 ≤ #14 < #15 = #16 + (-#17) + (~#18))
+
+/-- info: hl(if #1 then #2 else #3) : Exp -/
+#guard_msgs in
+#check hl(if #1 then #2 else #3)
+
+/-- info: hl((#1, #2, #3)) : Exp -/
+#guard_msgs in
+#check hl((#1, #2, #3))
+
+/--
+info: (Exp.val (Val.lit (@OfNat.ofNat BaseLit (nat_lit 1) (@instOfNatBaseLit (nat_lit 1))))).pair
+  ((Exp.val (Val.lit (@OfNat.ofNat BaseLit (nat_lit 2) (@instOfNatBaseLit (nat_lit 2))))).pair
+    (Exp.val (Val.lit (@OfNat.ofNat BaseLit (nat_lit 3) (@instOfNatBaseLit (nat_lit 3)))))) : Exp
+-/
+#guard_msgs in
+set_option pp.explicit true in
+#check hl((#1, #2, #3))
+
+/-- info: hl_val((#1, #BaseLit.unit, #(BaseLit.bool true), #(BaseLit.int (-1)))) : Val -/
+#guard_msgs in
+#check hl_val((#1, #(), #true, #(.int (-1))))
+
+/--
+info: (Val.lit (@OfNat.ofNat BaseLit (nat_lit 1) (@instOfNatBaseLit (nat_lit 1)))).pair
+  ((Val.lit (@OfNat.ofNat BaseLit (nat_lit 2) (@instOfNatBaseLit (nat_lit 2)))).pair
+    (Val.lit (@OfNat.ofNat BaseLit (nat_lit 3) (@instOfNatBaseLit (nat_lit 3))))) : Val
+-/
+#guard_msgs in
+set_option pp.explicit true in
+#check hl_val((#1, #2, #3))
+
+/-- info: hl(fst(snd((#1, #2, #3)))) : Exp -/
+#guard_msgs in
+#check hl(fst(snd((#1, #2, #3))))
+
+/-- info: hl(case: injl(injr(#1)) | _ => #1 | y => #2) : Exp -/
+#guard_msgs in
+#check hl(case: injl(injr(#1)) | _ => #1 | y => #2)
+
+/-- info: hl_val(injl(injr(#1))) : Val -/
+#guard_msgs in
+#check hl_val(injl(injr(#1)))
+
+
+/--
+info: hl(let x := ref(#0);
+    let y := allocn(!x, #0);
+      (x ← !x + #1); fork(cmpXchg(x, #1, #2); xchg(x, #2); faa(x, #4)); assert((!x = #0)); free(x)) : Exp
+-/
+#guard_msgs in
+#check hl(let x := ref(#0); let y := allocn(!x, #0); x ← !x + #1; fork(cmpXchg(x, #1, #2); xchg(x, #2); faa(x, #4)); assert(!x = #0); free(x))
+
+/--
+info: (Exp.rec_ Binder.anon (Binder.named "x")
+      ((Exp.rec_ Binder.anon (Binder.named "y")
+            ((Exp.rec_ Binder.anon Binder.anon
+                  ((Exp.rec_ Binder.anon Binder.anon
+                        ((Exp.rec_ Binder.anon Binder.anon (Exp.var "x").free).app
+                          (Exp.binop BinOp.eq (Exp.var "x").load
+                              (Exp.val
+                                (Val.lit
+                                  (@OfNat.ofNat BaseLit (nat_lit 0) (@instOfNatBaseLit (nat_lit 0)))))).assert)).app
+                    ((Exp.rec_ Binder.anon Binder.anon
+                            ((Exp.rec_ Binder.anon Binder.anon
+                                  ((Exp.var "x").faa
+                                    (Exp.val
+                                      (Val.lit
+                                        (@OfNat.ofNat BaseLit (nat_lit 4) (@instOfNatBaseLit (nat_lit 4))))))).app
+                              ((Exp.var "x").xchg
+                                (Exp.val
+                                  (Val.lit (@OfNat.ofNat BaseLit (nat_lit 2) (@instOfNatBaseLit (nat_lit 2)))))))).app
+                        ((Exp.var "x").cmpXchg
+                          (Exp.val (Val.lit (@OfNat.ofNat BaseLit (nat_lit 1) (@instOfNatBaseLit (nat_lit 1)))))
+                          (Exp.val
+                            (Val.lit (@OfNat.ofNat BaseLit (nat_lit 2) (@instOfNatBaseLit (nat_lit 2))))))).fork)).app
+              (Exp.binop BinOp.plus ((Exp.var "x").store (Exp.var "x").load)
+                (Exp.val (Val.lit (@OfNat.ofNat BaseLit (nat_lit 1) (@instOfNatBaseLit (nat_lit 1)))))))).app
+        ((Exp.var "x").load.allocN
+          (Exp.val (Val.lit (@OfNat.ofNat BaseLit (nat_lit 0) (@instOfNatBaseLit (nat_lit 0)))))))).app
+  ((Exp.val (Val.lit (@OfNat.ofNat BaseLit (nat_lit 1) (@instOfNatBaseLit (nat_lit 1))))).allocN
+    (Exp.val (Val.lit (@OfNat.ofNat BaseLit (nat_lit 0) (@instOfNatBaseLit (nat_lit 0)))))) : Exp
+-/
+#guard_msgs in
+set_option pp.explicit true in
+#check hl(let x := ref(#0); let y := allocn(!x, #0); x ← !x + #1; fork(cmpXchg(x, #1, #2); xchg(x, #2); faa(x, #4)); assert(!x = #0); free(x))
+
+end test
+end Notation
