Test/HeapLangExamples.lean
@@ -6,6 +6,8 @@ open ITree.Exec
 
 namespace HeapLang
 
+/-- TODO: have a better simp set -/
+
 example s :
   exec heaplangEH hl(#1 + #1).denote s λ t _ => t = return (.lit $ .int 2) := by
     simp [Exp.denote, Exp.isVal, BinOp.denote, BinOp.evalInt]
@@ -17,5 +19,18 @@ example tp heap :
     simp [Exp.denote, Exp.isVal, Exp.subst, Exp.substStr, yieldAfter, Exp.yieldIfNotVal, Val.rec!, BinOp.denote, BinOp.evalInt, -bind_pure_comp]
     apply exec_yield_same
     apply exec_yield_same
+    apply exec.stop
+    simp
+
+-- set_option pp.explicit true in
+example tp heap :
+  exec heaplangEH hl(let x := #1; assert(x + #1 = #2)).denote ⟨tp, heap⟩ λ t _ => t = return (.lit $ .unit) := by
+    simp [Exp.denote, Exp.assert, Val.isUnboxed, BaseLit.isUnboxed, Val.bool!, Exp.isVal, Exp.subst, Exp.substStr, yieldAfter, Exp.yieldIfNotVal, Val.rec!, BinOp.denote, BinOp.evalInt, -bind_pure_comp]
+    apply exec_yield_same
+    apply exec_yield_same
+    apply exec_yield_same
+    apply exec_yield_same
+    unfold instOfNatBaseLit
+    simp
     apply exec.stop
     simp
